src/tactics/FStar.Tactics.Hooks.fst
@@ -160,7 +160,7 @@ let by_tactic_interp (pol:pol) (e:Env.env) (t:term) : tres =
             when S.fv_eq_lid fv PC.rewrite_by_tactic_lid ->
 
         // Create a new uvar that must be equal to the initial term
-        let uvtm, _, g_imp = Env.new_implicit_var_aux "rewrite_with_tactic RHS" tm.pos e typ Strict None in
+        let uvtm, _, g_imp = Env.new_implicit_var_aux "rewrite_with_tactic RHS" tm.pos e typ Strict None false in
 
         let u = e.universe_of e typ in
         // eq2 is squashed already, so it's in Type0
@@ -1011,7 +1011,7 @@ let postprocess (env:Env.env) (tau:term) (typ:term) (tm:term) : term =
     //we know that tm:typ
     //and we have a goal that u == tm
     //so if we solve that equality, we don't need to retype the solution of `u : typ`
-    let uvtm, _, g_imp = Env.new_implicit_var_aux "postprocess RHS" tm.pos env typ (Allow_untyped "postprocess") None in
+    let uvtm, _, g_imp = Env.new_implicit_var_aux "postprocess RHS" tm.pos env typ (Allow_untyped "postprocess") None false in
 
     let u = env.universe_of env typ in
     // eq2 is squashed already, so it's in Type0
